theories/Infra/BoundedBelow.v
@@ -1,0 +1,38 @@
+Require Import Util CSet AnnP.
+
+Definition bounded_below
+           (c : nat)
+           (k : nat)
+  : ⦃nat⦄ -> Prop
+  :=
+    fun a => cardinal (filter (fun x => B[x <= c]) a) <= k.
+
+
+Instance bounded_in_equal_morph
+  : Proper (eq ==> eq ==> Equal ==> iff) bounded_below.
+Proof.
+  unfold Proper, respectful, bounded_below; intros; subst.
+  rewrite H1. reflexivity.
+Qed.
+
+Instance bounded_in_subset_morph
+  : Proper (eq ==> eq ==> Equal ==> impl) bounded_below.
+Proof.
+  unfold Proper, respectful, bounded_below, impl, flip; intros; subst.
+  rewrite <- H1. rewrite <- H2. reflexivity.
+Qed.
+
+
+Instance bounded_in_equal_ptw
+  : Proper (eq ==> eq ==> pointwise_relation _ iff) bounded_below.
+Proof.
+  unfold Proper, respectful, pointwise_relation; intros; subst.
+  reflexivity.
+Qed.
+
+Instance bounded_in_impl_ptw'
+  : Proper (eq ==> eq ==> pointwise_relation _ impl) bounded_below.
+Proof.
+  unfold Proper, respectful, pointwise_relation, impl, flip; intros; subst.
+  eauto.
+Qed.
