theories/Infra/InfinitePartition.v
@@ -1,0 +1,181 @@
+Require Import Util CSet Fresh.
+
+Set Implicit Arguments.
+
+Record inf_subset :=
+  {
+    inf_subset_P :> nat -> bool;
+    inf_subset_inf : forall x, exists y, inf_subset_P y /\ y > x
+  }.
+
+Hint Resolve inf_subset_inf.
+
+Record inf_partition :=
+  { part_1 : inf_subset;
+    part_2 : inf_subset;
+    part_disj : forall x, part_1 x -> part_2 x -> False;
+    part_cover : forall x, part_1 x + part_2 x;
+  }.
+
+Fixpoint even (n:nat) : bool :=
+  match n with
+  | 0 => true
+  | S 0 => false
+  | S (S n) => even n
+  end.
+
+Lemma even_or_successor x
+  : even x \/ even (1 + x).
+Proof.
+  induction x; eauto.
+  destruct IHx; eauto.
+Qed.
+
+Definition even_inf_subset : inf_subset.
+Proof.
+  refine (Build_inf_subset even _).
+  - intros. destruct (even_or_successor (S x)); eauto.
+    eexists (2+x); simpl; split; eauto.
+Defined.
+
+Definition odd := (fun x => negb (even x)).
+
+Lemma even_not_even x
+  : even x = negb (even (S x)).
+Proof.
+  general induction x; eauto.
+  - simpl even at 2.
+    destruct (even x); destruct (even (S x)); simpl in *; intuition.
+Qed.
+
+Definition odd_inf_subset : inf_subset.
+Proof.
+  refine (Build_inf_subset odd _).
+  - unfold odd. intros.
+    destruct (even_or_successor x); eauto.
+    + eexists (S x). rewrite <- even_not_even.
+      split; eauto.
+    + eexists (S (S x)); simpl.
+      rewrite even_not_even in H. eauto.
+Defined.
+
+Definition even_part : inf_partition.
+Proof.
+  refine (Build_inf_partition even_inf_subset odd_inf_subset _ _).
+  - intros.
+    unfold even_inf_subset in H. simpl in H.
+    unfold odd_inf_subset in H0. simpl in H0.
+    unfold odd in H0. unfold negb in H0. cases in H0; eauto.
+  - intros.
+    unfold even_inf_subset, odd_inf_subset, odd, negb; simpl.
+    cases; eauto.
+Qed.
+
+Require Import SafeFirst.
+
+Lemma fresh_variable_always_exists_in_inf_subset (lv:set nat) (p:inf_subset) n
+: safe (fun x => x ∉ lv /\ p x) n.
+Proof.
+  - decide (n > SetInterface.fold max lv 0).
+    + decide (p n).
+      * econstructor. split; eauto.
+        intro. exploit fresh_spec'; eauto.
+        Set Printing All. intros. omega.
+      * edestruct (inf_subset_inf p n); dcr.
+        eapply (@safe_antitone _ _ x);[|omega].
+        econstructor; split; eauto.
+        intro. exploit fresh_spec'; eauto. omega.
+    + decide (p (S (SetInterface.fold max lv 0))).
+      * eapply safe_antitone. instantiate (1:=S (SetInterface.fold max lv 0)).
+        econstructor. split; eauto. intro.
+        exploit fresh_spec'; eauto. omega.
+        omega.
+      * edestruct (inf_subset_inf p (S (SetInterface.fold Init.Nat.max lv 0)));
+          dcr.
+        eapply (@safe_antitone _ _ x);[|omega].
+        econstructor; split; eauto.
+        intro. exploit fresh_spec'; eauto. omega.
+Qed.
+
+Definition least_fresh_P (p:inf_subset) (lv:set nat) : nat.
+  refine (@safe_first (fun x => x ∉ lv /\ p x) _ 0 _).
+  - eapply fresh_variable_always_exists_in_inf_subset.
+Defined.
+
+
+
+Lemma semantic_branch (P Q:Prop) `{Computable Q}
+  : P \/ Q -> ((~ Q /\ P) \/ Q).
+Proof.
+  decide Q; clear H; intros; intuition.
+Qed.
+
+Lemma least_fresh_P_full_spec p G
+  : least_fresh_P p G ∉ G
+    /\ (forall m, p m ->  m < least_fresh_P p G -> m ∈ filter p G)
+    /\ p (least_fresh_P p G).
+Proof.
+  unfold least_fresh_P.
+  eapply safe_first_spec with
+  (I:= fun n => forall m, p m -> m < n -> m ∈ filter p G).
+  - intros; dcr. rewrite de_morgan_dec, <- in_dneg in H0.
+    destruct H0; dcr.
+    + decide (m = n); subst; eauto.
+      * cset_tac.
+      * exploit (H m); eauto. omega.
+    + decide (m = n); subst; eauto.
+      * cset_tac.
+      * exploit (H m); eauto. omega.
+  - intros. cset_tac.
+  - intros; omega.
+Qed.
+
+Definition least_fresh_part (p:inf_partition) (G:set nat) x :=
+  if part_1 p x then least_fresh_P (part_1 p) G
+  else least_fresh_P (part_2 p) G.
+
+Lemma least_fresh_part_fresh p G x
+  : least_fresh_part p G x ∉ G.
+Proof.
+  unfold least_fresh_part; cases; eauto.
+  - eapply least_fresh_P_full_spec.
+  - eapply least_fresh_P_full_spec.
+Qed.
+
+Lemma least_fresh_part_1 (p:inf_partition) G x
+  : part_1 p x
+    -> part_1 p (least_fresh_part p G x).
+Proof.
+  unfold least_fresh_part; intros; cases.
+  eapply least_fresh_P_full_spec.
+Qed.
+
+Lemma least_fresh_part_2 (p:inf_partition) G x
+  : part_2 p x
+    -> part_2 p (least_fresh_part p G x).
+Proof.
+  unfold least_fresh_part; intros. cases.
+  - exfalso. eapply part_disj; eauto.
+  - eapply least_fresh_P_full_spec.
+Qed.
+
+Lemma least_fresh_P_ext p (G G' : ⦃nat⦄)
+  : G [=] G' -> least_fresh_P p G = least_fresh_P p G'.
+Proof.
+  intros. unfold least_fresh_P; eauto.
+  eapply safe_first_ext. intros. rewrite H. reflexivity.
+Qed.
+
+Lemma least_fresh_part_ext p (G G' : ⦃nat⦄) x
+  : G [=] G' -> least_fresh_part p G x = least_fresh_part p G' x.
+Proof.
+  intros. unfold least_fresh_part; cases; eauto using least_fresh_P_ext.
+Qed.
+
+Lemma least_fresh_list_part_ext p n G G'
+  : G [=] G'
+    -> fresh_list_stable (least_fresh_part p) G n = fresh_list_stable (least_fresh_part p) G' n.
+Proof.
+  eapply fresh_list_stable_ext.
+  intros. eapply least_fresh_part_ext; eauto.
+Qed.
