theories/Infra/MapSep.v
@@ -1,0 +1,56 @@
+Require Import Util CSet InfinitePartition MapAgreement.
+
+Definition sep (p:inf_partition) (G:set nat) (ϱ:nat -> nat) :=
+  (forall x, x ∈ G -> part_1 p x -> part_1 p (ϱ x))
+  /\ (forall x, x ∈ G -> part_2 p x -> part_2 p (ϱ x)).
+
+Instance sep_morphism_impl
+  : Proper (eq ==> Equal ==> eq ==> impl) sep.
+Proof.
+  unfold Proper, respectful, impl. intros ? p ? x ? EQ ? ϱ ? SEP; subst.
+  destruct SEP; split; intros.
+  - eapply H; eauto. rewrite EQ; eauto.
+  - eapply H0; eauto. rewrite EQ; eauto.
+Qed.
+
+Instance sep_morphism_iff
+  : Proper (eq ==> Equal ==> eq ==> iff) sep.
+Proof.
+  unfold Proper, respectful; intros; subst.
+  split; rewrite H0; eauto.
+Qed.
+
+Instance sep_morphism_Subset_impl
+  : Proper (eq ==> Subset ==> eq ==> flip impl) sep.
+Proof.
+  unfold Proper, respectful, flip, impl; intros; subst.
+  destruct H2; split; intros; eauto.
+Qed.
+
+Instance sep_morphism_Subset_impl'
+  : Proper (eq ==> flip Subset ==> eq ==> impl) sep.
+Proof.
+  unfold Proper, respectful, flip, impl; intros; subst.
+  destruct H2; split; intros; eauto.
+Qed.
+
+Lemma sep_incl p lv lv' ϱ
+  : sep p lv ϱ
+    -> lv' ⊆ lv
+    -> sep p lv' ϱ.
+Proof.
+  intros A B. rewrite B; eauto.
+Qed.
+
+Lemma sep_agree p D ϱ ϱ'
+  : agree_on eq D ϱ ϱ'
+    -> sep p D ϱ
+    -> sep p D ϱ'.
+Proof.
+  intros AGR [GT LE]; split; intros.
+  - rewrite <- AGR; eauto.
+  - rewrite <- AGR; eauto.
+Qed.
+
+
+Hint Resolve sep_incl sep_agree.
